coqimp/contextswitch/proof/AdjustCWP.v
@@ -1,0 +1,385 @@
+Require Import Coqlib.                                         
+Require Import Maps.            
+Require Import LibTactics.   
+        
+Require Import Integers.  
+Open Scope Z_scope.        
+Import ListNotations.  
+   
+Set Asymmetric Patterns.  
+        
+Require Import state.    
+Require Import language. 
+ 
+Set Implicit Arguments.    
+Unset Strict Implicit. 
+               
+Require Import logic.
+    
+Require Import lemmas.
+Require Import lemmas_ins.
+
+Require Import Coq.Logic.FunctionalExtensionality.
+
+Require Import integer_lemma.
+
+Require Import sep_lemma.
+Require Import reg_lemma.
+Require Import derived_rule.
+
+Require Import tm_dly_lemma.
+
+Require Import code.
+Require Import ctxswitch_spec.
+
+Require Import lemma1.
+
+Open Scope nat.
+Open Scope code_scope.
+Open Scope mem_scope.
+
+Lemma in_range_0_7_num :
+  forall v,
+    $ 0 <=ᵤᵢ v <=ᵤᵢ $ 7 ->
+    v = ($ 0) \/ v = ($ 1) \/ v = ($ 2) \/ v = ($ 3) \/
+    v = ($ 4) \/ v = ($ 5) \/ v = ($ 6) \/ v = ($ 7).
+Proof.
+  intros.
+  rewrite <- Int.repr_unsigned with (i := v).
+  unfolds int_leu.
+  unfolds Int.ltu, Int.eq.
+  assert (Int.unsigned $ 0 = 0%Z); eauto.
+  assert (Int.unsigned $ 7 = 7%Z); eauto.
+  try rewrite H0 in *.
+  try rewrite H1 in *.
+  destruct v.
+  simpl Int.unsigned in *.
+  destruct (zlt 0 intval); destruct (zeq 0 intval);
+    destruct (zlt intval 7); destruct (zeq intval 7); subst; eauto;
+      tryfalse; try omega.
+  destruct intval; tryfalse; eauto 20.
+  do 3 (try destruct p; eauto 10; tryfalse).
+  do 7 right.
+  eauto.
+Qed.
+
+Lemma post_cwp_step_limit_8 :
+  forall id vi,
+    $ 0 <=ᵤᵢ id <=ᵤᵢ $ 7 -> $ 0 <=ᵤᵢ vi <=ᵤᵢ $ 7 ->
+    post_cwp id = vi \/ post_cwp (post_cwp id) = vi \/ post_cwp (post_cwp (post_cwp id)) = vi \/
+    post_cwp (post_cwp (post_cwp (post_cwp id))) = vi \/
+    post_cwp (post_cwp (post_cwp (post_cwp (post_cwp id)))) = vi \/
+    post_cwp (post_cwp (post_cwp (post_cwp (post_cwp (post_cwp id))))) = vi \/
+    post_cwp (post_cwp (post_cwp (post_cwp (post_cwp (post_cwp (post_cwp id)))))) = vi \/
+    post_cwp (post_cwp (post_cwp (post_cwp (post_cwp (post_cwp (post_cwp (post_cwp id))))))) = vi.
+Proof.
+  intros.
+  unfold post_cwp.
+  unfold Int.modu.
+  unfold Int.add.
+  unfold N.
+  unfolds int_leu.
+  unfolds Int.ltu.
+  unfolds Int.eq.
+  assert (Int.unsigned $ 0 = 0%Z); eauto.
+  assert (Int.unsigned $ 7 = 7%Z); eauto.
+  assert (Int.unsigned $ 1 = 1%Z); eauto.
+  assert (Int.unsigned $ 8 = 8%Z); eauto.
+  try rewrite H1 in *.
+  try rewrite H2 in *.
+  try rewrite H3 in *.
+  try rewrite H4 in *.
+  try rewrite <- Int.repr_unsigned with (i := id).
+  try rewrite <- Int.repr_unsigned with (i := vi).
+  destruct id, vi.
+  simpls Int.unsigned.
+  destruct (zlt 0 intval); destruct (zeq 0 intval);
+    destruct (zlt intval 7); destruct (zeq intval 7);
+      destruct (zlt 0 intval0); destruct (zeq 0 intval0);
+        destruct (zlt intval0 7); destruct (zeq intval0 7);
+          tryfalse; subst; eauto 200; try omega.
+  {
+    destruct intval, intval0; tryfalse; eauto. 
+    do 4 (try destruct p; tryfalse; simpl; eauto 200);
+      do 4 (try destruct p0; tryfalse; simpl; eauto 200).
+  }
+  {
+    destruct intval; tryfalse; eauto.
+    do 4 (try destruct p; tryfalse; simpl; eauto 200).
+  }
+  {
+    destruct intval; tryfalse; eauto.
+    do 4 (try destruct p; tryfalse; simpl; eauto 200).
+  }
+  {
+    destruct intval0; tryfalse; eauto.
+    do 4 (try destruct p; tryfalse; simpl; eauto 200).
+  }
+  {
+    destruct intval0; tryfalse; eauto.
+    do 4 (try destruct p; tryfalse; simpl; eauto 200).
+  }
+Qed.
+  
+(*+ Lemmas for Integer +*)
+Lemma in_range_0_7_and_255_stable :
+  forall v,
+    $ 0 <=ᵤᵢ v <=ᵤᵢ $ 7 ->
+    ($ 255) &ᵢ (($ 1) <<ᵢ v) = ($ 1) <<ᵢ v.
+Proof.
+  intros.
+  unfolds int_leu.
+  unfolds Int.ltu.
+  unfolds Int.eq.
+  unfold Int.and.
+  unfold Int.shl.
+  assert (Int.unsigned $ 0 = 0%Z).
+  eauto.
+  assert (Int.unsigned $ 1 = 1%Z).
+  eauto.
+  assert (Int.unsigned $ 7 = 7%Z).
+  eauto.
+  assert (Int.unsigned $ 255 = 255%Z).
+  eauto.
+  try rewrite H0 in *.
+  try rewrite H1 in *.
+  try rewrite H2 in *.
+  try rewrite H3 in *.
+  destruct v.
+  simpl Int.unsigned in *.
+  destruct (zlt 0 intval); destruct (zeq 0 intval);
+    destruct (zlt intval 7); destruct (zeq intval 7);
+      tryfalse; subst; eauto; try omega.
+  destruct intval; tryfalse.
+  do 3 (destruct p; tryfalse; eauto).
+Qed.
+  
+Lemma in_range_0_7_and :
+  forall x v,
+    $ 0 <=ᵤᵢ v <=ᵤᵢ $ 7 ->
+    x &ᵢ (($ 1) <<ᵢ v) = (get_range 0 7 x) &ᵢ (($ 1) <<ᵢ v).
+Proof. 
+  intros.
+  unfold get_range.
+  simpl.
+  rewrite Int.shl_zero.
+  assert ((($ 1) <<ᵢ ($ 8)) -ᵢ ($ 1) = ($ 255)).
+  eauto.
+  rewrite H0.
+  rewrite Int.and_assoc.
+  rewrite in_range_0_7_and_255_stable; eauto.
+Qed.
+
+Lemma get_range_0_7_or :
+  forall x y,
+    get_range 0 7 (x |ᵢ y) = (get_range 0 7 x) |ᵢ (get_range 0 7 y).
+Proof. 
+  intros.
+  unfold get_range.
+  simpl.
+  rewrite Int.shl_zero.
+  assert ((($ 1) <<ᵢ ($ 8)) -ᵢ ($ 1) = ($ 255)).
+  eauto.
+  rewrite H.
+  rewrite Int.and_or_distrib_l; eauto.
+Qed.
+
+Inductive rotate : Word -> Word -> Word -> Word -> Prop :=
+| rotate_end :
+    forall (oid oid vi l : Word),
+      rotate oid oid vi (($ 1) <<ᵢ oid)
+| rotate_cons :
+    forall (oid id vi l : Word),
+      rotate oid id vi l -> post_cwp id <> vi -> $ 0 <=ᵤᵢ id <=ᵤᵢ $ 7 ->
+      rotate oid (post_cwp id) vi ((($ 1) <<ᵢ l |ᵢ l >>ᵢ ($ 7))).
+
+Lemma rotate_no_reach :
+  forall oid id vi l,
+    $ 0 <=ᵤᵢ oid <=ᵤᵢ $ 7 -> $ 0 <=ᵤᵢ vi <=ᵤᵢ $ 7 -> $ 0 <=ᵤᵢ id <=ᵤᵢ $ 7 -> rotate oid id vi l ->
+    l <> ($ 15) <<ᵢ ($ 1) |ᵢ ($ 7) <<ᵢ ($ 1).
+Proof.
+  intros.
+  inversion H2; subst.
+  {
+    intro.
+    eapply in_range_0_7_num in H.
+    do 7 (destruct H as [a | H]; [subst; tryfalse | idtac]).
+    subst; tryfalse.
+  }
+
+  inversion H3; subst.
+  {
+    intro.
+    eapply in_range_0_7_num in H.
+    do 7 (destruct H as [a | H]; [subst; tryfalse | idtac]).
+    subst; tryfalse.
+  }
+ 
+  inversion H6; subst.
+  { 
+    intro.
+    eapply in_range_0_7_num in H.
+    do 7 (destruct H as [a | H]; [subst; tryfalse | idtac]).
+    subst; tryfalse.
+  }
+ 
+  inversion H9; subst.
+  {
+    intro.
+    eapply in_range_0_7_num in H.
+    do 7 (destruct H as [a | H]; [subst; tryfalse | idtac]).
+    subst; tryfalse.
+  }
+
+  inversion H12; subst.
+  {
+    intro.
+    eapply in_range_0_7_num in H.
+    do 7 (destruct H as [a | H]; [subst; tryfalse | idtac]).
+    subst; tryfalse.
+  }
+
+  inversion H15; subst.
+  {
+    intro.
+    eapply in_range_0_7_num in H.
+    do 7 (destruct H as [a | H]; [subst; tryfalse | idtac]).
+    subst; tryfalse.
+  }
+
+  inversion H18; subst.
+  {
+    intro.
+    eapply in_range_0_7_num in H.
+    do 7 (destruct H as [a | H]; [subst; tryfalse | idtac]).
+    subst; tryfalse.
+  }
+
+  inversion H21; subst.
+  {
+    intro.
+    eapply in_range_0_7_num in H.
+    do 7 (destruct H as [a | H]; [subst; tryfalse | idtac]).
+    subst; tryfalse.
+  }
+
+  inversion H24; subst.
+  {
+    intro.
+    eapply in_range_0_7_num in H.
+    do 7 (destruct H as [a | H]; [subst; tryfalse | idtac]).
+    subst; tryfalse.
+  }
+   
+  clear - H29 H0 H22 H16 H10 H16 H7 H19 H13 H20 H25 H28.
+  false. 
+  eapply post_cwp_step_limit_8 with (vi := vi) in H29; eauto.
+  do 7 (destruct H29 as [a | H29]; [tryfalse | idtac]).
+  tryfalse.
+Qed.
+  
+(*+ Proof +*)
+Theorem Ta0AdjustCWPProof :
+  forall vl,
+    spec |- {{ ta0_adjust_cwp_pre vl }}
+             ta0_adjust_cwp
+           {{ ta0_adjust_cwp_post vl }}.
+Proof.
+  intros.
+  unfold ta0_adjust_cwp_pre.
+  unfold ta0_adjust_cwp_post.
+  hoare_ex_intro_pre.
+  renames x' to fmg, x'0 to fmo, x'1 to fml, x'2 to fmi.
+  renames x'3 to id, x'6 to vi, x'4 to F, x'5 to vy. 
+  renames x'8 to i, x'13 to vz, x'14 to vn.
+  renames x'7 to ll, x'9 to ct, x'10 to nt, x'11 to nctx, x'12 to nstk.
+  eapply Pure_intro_rule.
+  introv Hlgvl.
+  hoare_lift_pre 13.
+  eapply Pure_intro_rule.
+  introv Hpure.
+  hoare_lift_pre 13.
+  eapply Pure_intro_rule.
+  introv Hnctx.
+  destruct fmg, fmo, fml, fmi.
+  eapply backward_rule.
+  introv Hs.
+  simpl_sep_liftn_in Hs 2.
+  eapply Regs_Global_combine_GenRegs in Hs; eauto.
+  unfold ta0_adjust_cwp.
+ 
+  destruct Hpure as [Hg4 [Hid [Hg4_hid [ Hg7 Hct ] ] ] ].
+  simpl in Hg4.
+  inversion Hg4; subst.
+  simpl in Hg7.
+  inversion Hg7; subst.
+
+  (** sll g4 1 g5 *)
+  eapply seq_rule.
+  TimReduce_simpl.
+  eapply sll_rule_reg; eauto.
+  simpl; eauto.
+  rewrite in_range1; eauto.
+  simpl upd_genreg.
+
+  (** srl g4 (OS_WINDOWS - 1) g5 *)
+  unfold OS_WINDOWS.
+  assert (Heq7 : ($ 8) -ᵢ ($ 1) = ($ 7)).
+  eauto.
+  rewrite Heq7.
+  eapply seq_rule.
+  TimReduce_simpl.
+  eapply srl_rule_reg; eauto.
+  simpl; eauto.
+  rewrite in_range7; eauto.
+  simpl upd_genreg. 
+  rewrite get_range_0_4_stable; eauto.
+  rewrite get_range_0_4_stable; eauto.
+  
+  (** or g4 g5 g4 *)
+  eapply seq_rule.
+  TimReduce_simpl.
+  eapply or_rule_reg; eauto.
+  simpl; eauto. 
+  simpl upd_genreg.
+
+  eapply hoare_pure_gen' with (pu := $ 0 <=ᵤᵢ id <=ᵤᵢ $ 7 /\ $ 0 <=ᵤᵢ vi <=ᵤᵢ $ 7).
+  {
+    introv Hs.
+    simpl_sep_liftn_in Hs 2.
+    unfold FrameState in Hs.
+    asrt_to_line_in Hs 3.
+    simpl_sep_liftn_in Hs 4.
+    eapply sep_pure_l_elim in Hs; eauto.
+    simpljoin1; eauto.
+  } 
+  eapply Pure_intro_rule.
+  introv Hid_inrange.
+  destruct Hid_inrange as [Hid_inrange Hvi_inrange].
+    
+  (** andcc g4 g7 g0 *)
+  hoare_lift_pre 4.
+  hoare_lift_pre 5.
+  hoare_lift_pre 3.
+  eapply seq_rule.
+  TimReduce_simpl. 
+  eapply andcc_rule_reg; eauto.
+  simpl upd_genreg.
+  simpl get_genreg_val.
+  assert (Hiszero : iszero ((i >>ᵢ ($ 7)) |ᵢ (i <<ᵢ ($ 1))) &ᵢ (($ 1) <<ᵢ vi) =
+         iszero (get_range 0 7 ((i >>ᵢ ($ 7)) |ᵢ (i <<ᵢ ($ 1)))) &ᵢ (($ 1) <<ᵢ vi)).
+  {
+    rewrite in_range_0_7_and; eauto.
+  }
+  
+  rewrite Hiszero.
+
+  Lemma tst :
+    forall i,
+      
+  
+  rewrite get_range_0_7_or.
+  Search Int.shl.
+  
+    
+  >>>>>>>>>>>>>>>>>>
